src/dev/ai4fm/heap_example.thy
@@ -1,0 +1,206 @@
+theory heap_example
+imports "ai4fm_setup" "heap/HEAP1" "heap/HEAP1Lemmas"
+begin  
+
+
+ML{*
+  (* define your local path here *)
+  val pspath = OS.FileSys.getDir() ^ "/Workspace/StrategyLang/psgraph/src/dev/ai4fm/"
+  val pre_post_file = "heap_pre_post.psgraph"
+  val hca_file = "heap_hca.psgraph"
+  val onep_file = "heap_onep.psgraph"
+  val structure_file = "heap_structure.psgraph"
+  val rippling_file = "heap_rippling.psgraph"; 
+  val demo_rippling_file = "rippling/rippling.psgraph" 
+
+ 
+  val clause_def = "";
+  val data =  data   
+  |> Clause_GT.update_data_defs (fn x => (Clause_GT.scan_data IsaProver.default_ctxt clause_def) @ x);
+
+  val demo_rippling =  PSGraph.read_json_file (SOME data) (pspath ^ demo_rippling_file);
+  val pre_post = PSGraph.read_json_file (SOME data) (pspath ^ pre_post_file);
+  val hca = PSGraph.read_json_file (SOME data) (pspath ^ hca_file);
+  val onep = PSGraph.read_json_file (SOME data) (pspath ^ onep_file);
+  val struct_break = PSGraph.read_json_file (SOME data) (pspath ^ structure_file);
+  val rippling = PSGraph.read_json_file (SOME data) (pspath ^ rippling_file);
+*}
+
+setup {* PSGraphIsarMethod.add_graph ("demo_rippling", demo_rippling) *}
+setup {* PSGraphIsarMethod.add_graph ("pre_post", pre_post) *}
+setup {* PSGraphIsarMethod.add_graph ("hca", hca) *}
+setup {* PSGraphIsarMethod.add_graph ("onep", onep) *}
+setup {* PSGraphIsarMethod.add_graph ("struct_break", struct_break) *}
+setup {* PSGraphIsarMethod.add_graph ("rippling", demo_rippling) *}
+
+thm F1_inv_def
+thm Disjoint_def
+thm sep_def
+thm nat1_map_def
+
+thm VDMMaps.l_dom_dom_ar
+declare  VDMMaps.l_dom_dom_ar [wrule]
+lemma finite_Diff[wrule]: "finite A \<Longrightarrow> finite (A - B) = finite A"
+by (metis finite_Diff)
+
+(* the first simple rippling example in the book *)
+lemma "finite (dom(f)) \<and> the (f(r)) \<noteq> s \<and> nat1 s \<and> r \<in> dom(f) \<and> s \<le> the(f(r)) \<Longrightarrow> finite(dom({r} -\<triangleleft> f))"
+apply (elim conjE)+ 
+ML_val {*-
+  val st =  Thm.cprem_of (#goal @{Isar.goal}) 1 |> Thm.term_of;
+  val ps_thm = Tinker.start_ieval @{context} (SOME rippling) (SOME []) (SOME st) (* prove the goal *)
+          |> EData.get_pplan |> IsaProver.get_goal_thm(* get the theorem *)
+*}
+apply (tinker rippling)
+done
+
+
+ML{*-
+TextSocket.safe_close();
+*}
+
+thm l_disjoint_dispose1_ext
+lemma dummy: "(x = x) = True"  by auto
+lemma dummy2: "(A \<and> True) = A"  by auto
+
+lemma "l \<in> dom (S -\<triangleleft> f) \<Longrightarrow> ((S -\<triangleleft> f) l) = (f l)"
+ by (rule VDMMaps.f_in_dom_ar_apply_subsume)
+
+(*declare VDMMaps.f_in_dom_ar_apply_subsume [wrule]*)
+declare VDMMaps.f_in_dom_ar_the_subsume [wrule]
+
+(* Now move on to the real heap example *)
+(* The PO of new fsb *)
+context level1_new
+begin
+lemmas pre_def = PO_new1_feasibility_def new1_pre_def
+lemmas post_def = new1_postcondition_def new1_post_def new1_post_eq_def new1_post_gr_def Set.Ball_def Set.Bex_def
+lemmas inv_def = F1_inv_def Disjoint_def  Set.Ball_def
+theorem locale1_new_FSB: "PO_new1_feasibility"
+(* setup the goal *)
+apply (insert l1_new1_precondition_def l1_invariant_def)
+
+(* Pattern: unfolding pre and post -- structure bd*)
+ML_val {*-
+  val st =  Thm.cprem_of (#goal @{Isar.goal}) 1 |> Thm.term_of;
+  val ps_thm = Tinker.start_ieval @{context} (SOME pre_post) (SOME []) (SOME st) (* prove the goal *)
+          |> EData.get_pplan |> IsaProver.get_goal_thm(* get the theorem *)
+*}
+apply (tinker pre_post) 
+apply (elim exE conjE)
+
+(* Move disj up *)
+(* GT def
+need_move_dis_up :- inst2(concl,"\<exists>x.?P x \<and> ?Q x", X, _), match(X, "?P \<or> ?Q").
+need_move_dis_up :- inst2(concl,"\<exists>x.?P x \<and> ?Q x", _, Y), match(Y, "?P \<or> ?Q").
+
+
+*)
+
+
+thm HOL.conj_disj_distribR HOL.ex_disj_distrib
+apply (subst HOL.conj_disj_distribR)
+apply (subst HOL.ex_disj_distrib)+
+
+(* Pattern: hca *)
+ML_val {*-
+  val st =  Thm.cprem_of (#goal @{Isar.goal}) 1 |> Thm.term_of;
+  val ps_thm = Tinker.start_ieval @{context} (SOME hca) (SOME []) (SOME st) (* prove the goal *)
+          |> EData.get_pplan |> IsaProver.get_goal_thm(* get the theorem *)
+*}
+apply (tinker hca)
+
+(* Manual steps:  Disj Intro and ex instantiation *)
+apply (rule disjI1) prefer 2
+apply (rule disjI2) prefer 2
+
+(* now part of one point rule*)
+apply (subst ex_comm) apply (rule_tac x = x in exI) prefer 2
+apply (subst ex_comm) apply (rule_tac x = x in exI) prefer 2
+
+(* Pattern: one point rule *)
+ML_val {*-
+  val st =  Thm.cprem_of (#goal @{Isar.goal}) 1 |> Thm.term_of;
+  val ps_thm = Tinker.start_ieval @{context} (SOME onep) (SOME []) (SOME st) (* prove the goal *)
+          |> EData.get_pplan |> IsaProver.get_goal_thm(* get the theorem *)
+*} 
+apply (tinker onep)
+
+(* from here, only prove part of the PO, ignore other subgoals *) 
+
+(* structure breakdown ? donesn't seem to fit here, only unfolding the inv_def *)
+unfolding inv_def
+apply (elim conjE)+ apply (intro conjI)+
+(* some simple sg are dischared by assumption*)
+apply assumption 
+apply assumption 
+apply (rule refl)
+
+(* now all remaining sgs are inv, and the other case *)
+(* the sg we now deal with is the INV disjoint *)
+(* pre tidy up for rippling , these steps can be potentially pwf for rippling *)
+thm VDMMaps.l_dom_dom_ar
+thm Set.Diff_iff
+apply (subst VDMMaps.l_dom_dom_ar)+
+apply (subst Set.Diff_iff)+
+apply (intro allI impI)+
+apply (elim conjE)+
+apply (erule_tac x = xa in allE )
+(* pwf for imp *) apply (erule impE) apply assumption
+(* elim allE for the inv hyp *) apply (erule_tac x = xb in allE)
+(* pwf for imp *) apply (erule impE) apply assumption
+(* pwf for imp *) apply (erule impE) apply assumption
+
+(* a bit more tidy up on the definition of Locs_of *)
+apply (subst  l_locs_of_Locs_of_iff)
+apply (metis l_in_dom_ar)
+apply (subst  l_locs_of_Locs_of_iff) apply (metis l_in_dom_ar)
+apply (subst(asm)  l_locs_of_Locs_of_iff) apply metis
+apply (subst(asm)  l_locs_of_Locs_of_iff) apply metis
+
+(* rippling *)
+thm VDMMaps.f_in_dom_ar_the_subsume 
+ML_val {*-
+  val st =  Thm.cprem_of (#goal @{Isar.goal}) 1 |> Thm.term_of;
+  val ps_thm = Tinker.start_ieval @{context} (SOME rippling) (SOME []) (SOME st) (* prove the goal *)
+          |> EData.get_pplan |> IsaProver.get_goal_thm(* get the theorem *)
+*} 
+
+
+apply (subst VDMMaps.f_in_dom_ar_apply_subsume)apply (metis l_in_dom_ar)
+apply (subst VDMMaps.f_in_dom_ar_apply_subsume) apply (metis l_in_dom_ar)
+apply assumption
+
+
+(* alternatiely, we can show the seq inv *)
+unfolding sep_def Ball_def
+apply (intro allI impI)
+apply (rotate_tac -4)
+apply( erule_tac x = xa in allE)
+apply (elim impE) apply (metis l_dom_ar_not_in_dom)
+(* rippling *)
+apply (subst VDMMaps.l_dom_dom_ar)+
+
+
+ML_val {*-
+  val st =  Thm.cprem_of (#goal @{Isar.goal}) 1 |> Thm.term_of;
+  val ps_thm = Tinker.start_ieval @{context} (SOME rippling) (SOME []) (SOME st) (* prove the goal *)
+          |> EData.get_pplan |> IsaProver.get_goal_thm(* get the theorem *)
+*}
+oops
+
+end
+
+
+context level1_dispose
+begin
+
+theorem locale1_dispose_FSB: "PO_dispose1_feasibility"
+
+unfolding PO_dispose1_feasibility_def dispose1_postcondition_def
+apply (insert  l1_invariant_def)
+apply (simp add: dispose1_equiv)
+unfolding dispose1_post2_def F1_inv_def
+oops
+end
+end
